theories/kcas/kcas.v
@@ -3,6 +3,10 @@ From iris.base_logic Require Import
 
 From zoo Require Import
   prelude.
+From zoo.common Require Import
+  list.
+From zoo.iris.bi Require Import
+  big_op.
 From zoo.iris.base_logic Require Import
   lib.twins
   lib.auth_mono
@@ -22,22 +26,232 @@ From kcas Require Export
 From zoo Require Import
   options.
 
+Implicit Types full : bool.
 Implicit Types i : nat.
 Implicit Types l loc casn : location.
-Implicit Types id : identifier.
-Implicit Types status : val.
+Implicit Types gid : identifier.
+Implicit Types v state cass : val.
+Implicit Types waiters : gmap gname nat.
+
+Axiom wp_equal : ∀ `{zoo_G : !ZooG Σ} v1 v2 E Φ,
+  ▷ Φ #(bool_decide (v1 = v2)) ⊢
+  WP v1 == v2 @ E {{ Φ }}.
+
+#[local] Program Definition kcas_prophet := {|
+  typed_prophet_type :=
+    identifier * bool ;
+  typed_prophet_of_val v :=
+    match v with
+    | ValTuple [ValProph gid; ValBool b] =>
+        Some (gid, b)
+    | _ =>
+        None
+    end ;
+  typed_prophet_to_val '(gid, b) :=
+    (#gid, #b)%V ;
+|}.
+Solve Obligations of kcas_prophet with
+  try done.
+Next Obligation.
+  intros (gid & b) v ->. done.
+Qed.
+Implicit Types prophs : list kcas_prophet.(typed_prophet_type).
+
+Definition kcas_loc_meta : Type :=
+  gname.
+Implicit Types γ : kcas_loc_meta.
+
+Record kcas_descr := {
+  kcas_descr_loc : location ;
+  kcas_descr_meta : kcas_loc_meta ;
+  kcas_descr_before : val ;
+  kcas_descr_after : val ;
+  kcas_descr_state : block_id ;
+}.
+Implicit Types descr : kcas_descr.
+
+#[local] Instance kcas_descr_inhabited : Inhabited kcas_descr :=
+populate {|
+    kcas_descr_loc := inhabitant ;
+    kcas_descr_meta := inhabitant ;
+    kcas_descr_before := inhabitant ;
+    kcas_descr_after := inhabitant ;
+    kcas_descr_state := inhabitant ;
+  |}.
+#[local] Instance kcas_descr_eq_dec : EqDecision kcas_descr :=
+  ltac:(solve_decision).
+#[local] Instance kcas_descr_countable :
+  Countable kcas_descr.
+Proof.
+  pose encode descr := (
+    descr.(kcas_descr_loc),
+    descr.(kcas_descr_meta),
+    descr.(kcas_descr_before),
+    descr.(kcas_descr_after),
+    descr.(kcas_descr_state)
+  ).
+  pose decode := λ '(loc, γ, before, after, state), {|
+    kcas_descr_loc := loc ;
+    kcas_descr_meta := γ ;
+    kcas_descr_before := before ;
+    kcas_descr_after := after ;
+    kcas_descr_state := state ;
+  |}.
+  refine (inj_countable' encode decode _). intros []. done.
+Qed.
+
+#[local] Definition kcas_state casn descr : val :=
+  ‘0@descr.(kcas_descr_state)(
+    #casn,
+    descr.(kcas_descr_before),
+    descr.(kcas_descr_after)
+  ).
+
+Inductive kcas_status :=
+  | KcasUndetermined
+  | KcasBefore
+  | KcasAfter.
+Implicit Types status : kcas_status.
+
+Record kcas_casn_meta := {
+  kcas_casn_meta_descrs : list kcas_descr ;
+  kcas_casn_meta_prophet : prophet_id ;
+  kcas_casn_meta_prophs : list kcas_prophet.(typed_prophet_type) ;
+  kcas_casn_meta_undetermined : block_id ;
+  kcas_casn_meta_post : gname ;
+  kcas_casn_meta_lstatus : gname ;
+  kcas_casn_meta_witnesses : list gname ;
+  kcas_casn_meta_waiters : gname ;
+  kcas_casn_meta_winning : gname ;
+  kcas_casn_meta_owner : gname ;
+}.
+Implicit Types η : kcas_casn_meta.
+
+#[local] Instance kcas_casn_meta_inhabited : Inhabited kcas_casn_meta :=
+  populate {|
+    kcas_casn_meta_descrs := inhabitant ;
+    kcas_casn_meta_prophet := inhabitant ;
+    kcas_casn_meta_prophs := inhabitant ;
+    kcas_casn_meta_undetermined := inhabitant ;
+    kcas_casn_meta_post := inhabitant ;
+    kcas_casn_meta_lstatus := inhabitant ;
+    kcas_casn_meta_witnesses := inhabitant ;
+    kcas_casn_meta_waiters := inhabitant ;
+    kcas_casn_meta_winning := inhabitant ;
+    kcas_casn_meta_owner := inhabitant ;
+  |}.
+#[local] Instance kcas_casn_meta_eq_dec : EqDecision kcas_casn_meta :=
+  ltac:(solve_decision).
+#[local] Instance kcas_casn_meta_countable :
+  Countable kcas_casn_meta.
+Proof.
+  pose encode η := (
+    η.(kcas_casn_meta_descrs),
+    η.(kcas_casn_meta_prophet),
+    η.(kcas_casn_meta_prophs),
+    η.(kcas_casn_meta_undetermined),
+    η.(kcas_casn_meta_post),
+    η.(kcas_casn_meta_lstatus),
+    η.(kcas_casn_meta_witnesses),
+    η.(kcas_casn_meta_waiters),
+    η.(kcas_casn_meta_winning),
+    η.(kcas_casn_meta_owner)
+  ).
+  pose decode := λ '(descrs, prophet, prophs, undetermined, post, lstatus, witnesses, waiters, winning, owner), {|
+    kcas_casn_meta_descrs := descrs ;
+    kcas_casn_meta_prophet := prophet ;
+    kcas_casn_meta_prophs := prophs ;
+    kcas_casn_meta_undetermined := undetermined ;
+    kcas_casn_meta_post := post ;
+    kcas_casn_meta_lstatus := lstatus ;
+    kcas_casn_meta_witnesses := witnesses ;
+    kcas_casn_meta_waiters := waiters ;
+    kcas_casn_meta_winning := winning ;
+    kcas_casn_meta_owner := owner ;
+  |}.
+  refine (inj_countable' encode decode _). intros []. done.
+Qed.
+
+#[local] Definition kcas_casn_meta_size η :=
+  length η.(kcas_casn_meta_descrs).
+#[local] Definition kcas_casn_meta_cass casn η :=
+  (λ descr,
+    (#descr.(kcas_descr_loc), kcas_state casn descr)%V
+  ) <$> η.(kcas_casn_meta_descrs).
+#[local] Definition kcas_casn_meta_outcome η :=
+  hd inhabitant η.(kcas_casn_meta_prophs).
+#[local] Definition kcas_casn_meta_winner η :=
+  (kcas_casn_meta_outcome η).1.
+#[local] Definition kcas_casn_meta_success η :=
+  (kcas_casn_meta_outcome η).2.
+#[local] Definition kcas_casn_meta_final η :=
+  if kcas_casn_meta_success η then KcasAfter else KcasBefore.
+
+#[local] Instance kcas_status_inhabited : Inhabited kcas_status :=
+  populate KcasUndetermined.
+
+#[local] Definition kcas_status_to_val casn η status : val :=
+  match status with
+  | KcasUndetermined =>
+      ‘Undetermined@η.(kcas_casn_meta_undetermined)( lst_to_val $ kcas_casn_meta_cass casn η )
+  | KcasBefore =>
+      §Before
+  | KcasAfter =>
+      §After
+  end.
 
 Inductive kcas_lstatus :=
-  | KcasUndetermined i
+  | KcasRunning i
   | KcasFinished.
 Implicit Types lstatus : kcas_lstatus.
 
+#[local] Instance kcas_lstatus_inhabited : Inhabited kcas_lstatus :=
+  populate KcasFinished.
+
 Inductive kcas_lstep : kcas_lstatus → kcas_lstatus → Prop :=
   | kcas_lstep_incr i :
-      kcas_lstep (KcasUndetermined i) (KcasUndetermined (S i))
+      kcas_lstep (KcasRunning i) (KcasRunning (S i))
   | kcas_lstep_finish i :
-      kcas_lstep (KcasUndetermined i) KcasFinished.
+      kcas_lstep (KcasRunning i) KcasFinished.
 #[local] Hint Constructors kcas_lstep : core.
+
+#[local] Lemma kcas_lsteps_running0 lstatus :
+  rtc kcas_lstep (KcasRunning 0) lstatus.
+Proof.
+  destruct lstatus as [i |].
+  - induction i; first done.
+    eapply rtc_r; [done | constructor].
+  - apply rtc_once. done.
+Qed.
+#[local] Lemma kcas_lstep_finished lstatus :
+  ¬ kcas_lstep KcasFinished lstatus.
+Proof.
+  inversion 1.
+Qed.
+#[local] Lemma kcas_lsteps_finished lstatus :
+  rtc kcas_lstep KcasFinished lstatus →
+  lstatus = KcasFinished.
+Proof.
+  inversion 1 as [| ? ? ? []] => //.
+Qed.
+#[local] Lemma kcas_lsteps_le lstatus1 i1 lstatus2 i2 :
+  rtc kcas_lstep lstatus1 lstatus2 →
+  lstatus1 = KcasRunning i1 →
+  lstatus2 = KcasRunning i2 →
+  i1 ≤ i2.
+Proof.
+  intros Hlsteps. move: i1. induction Hlsteps as [lstatus | lstatus1 ? lstatus2 Hlstep Hlsteps IH] => i1.
+  - naive_solver.
+  - intros -> ->. invert Hlstep.
+    + specialize (IH (S i1)). lia.
+    + apply kcas_lsteps_finished in Hlsteps as [=].
+Qed.
+
+#[local] Definition kcas_descr_final descr η :=
+  if kcas_casn_meta_success η then
+    descr.(kcas_descr_after)
+  else
+    descr.(kcas_descr_before).
 
 Class KcasG Σ `{zoo_G : !ZooG Σ} := {
   #[local] kcas_G_model_G :: TwinsG Σ val_O ;
@@ -70,164 +284,41 @@ Section kcas_G.
 
   Implicit Types P Q : iProp Σ.
 
-  #[local] Program Definition kcas_prophet := {|
-    typed_prophet_type :=
-      identifier * bool ;
-    typed_prophet_of_val v :=
-      match v with
-      | ValTuple [ValProph id; ValBool b] =>
-          Some (id, b)
-      | _ =>
-          None
-      end ;
-    typed_prophet_to_val '(id, b) :=
-      (#id, #b)%V ;
-  |}.
-  Solve Obligations of kcas_prophet with
-    try done.
-  Next Obligation.
-    intros (id & b) v ->. done.
-  Qed.
-
-  Definition kcas_loc_meta : Type :=
-    gname.
-  Implicit Types γ : kcas_loc_meta.
-
   #[local] Definition kcas_model₁ γ v :=
     twins_twin1 γ (DfracOwn 1) v.
   #[local] Definition kcas_model₂ γ v :=
     twins_twin2 γ v.
 
-  Record kcas_descr := {
-    kcas_descr_loc : location ;
-    kcas_descr_meta : kcas_loc_meta ;
-    kcas_descr_before : val ;
-    kcas_descr_after : val ;
-  }.
-
-  #[local] Instance kcas_descr_eq_dec : EqDecision kcas_descr :=
-    ltac:(solve_decision).
-  #[local] Instance kcas_descr_countable :
-    Countable kcas_descr.
-  Proof.
-    pose encode descr := (
-      descr.(kcas_descr_loc),
-      descr.(kcas_descr_meta),
-      descr.(kcas_descr_before),
-      descr.(kcas_descr_after)
-    ).
-    pose decode := λ '(loc, γ, before, after), {|
-      kcas_descr_loc := loc ;
-      kcas_descr_meta := γ ;
-      kcas_descr_before := before ;
-      kcas_descr_after := after ;
-    |}.
-    refine (inj_countable' encode decode _). intros []. done.
-  Qed.
-
-  Record kcas_casn_meta := {
-    kcas_casn_meta_descrs : list kcas_descr ;
-    kcas_casn_meta_prophet : prophet_id ;
-    kcas_casn_meta_prophs : list kcas_prophet.(typed_prophet_type) ;
-    kcas_casn_meta_undetermined : block_id ;
-    kcas_casn_meta_post : gname ;
-    kcas_casn_meta_lstatus : gname ;
-    kcas_casn_meta_witnesses : list gname ;
-    kcas_casn_meta_waiters : gname ;
-    kcas_casn_meta_winning : gname ;
-    kcas_casn_meta_owner : gname ;
-  }.
-  Implicit Types η : kcas_casn_meta.
-
-  #[local] Definition kcas_casn_meta_size η :=
-    length η.(kcas_casn_meta_descrs).
-  #[local] Definition kcas_casn_meta_cass casn η :=
-    (λ descr,
-      ( #descr.(kcas_descr_loc),
-        (#casn, descr.(kcas_descr_before), descr.(kcas_descr_after))
-      )%V
-    ) <$> η.(kcas_casn_meta_descrs).
-  #[local] Definition kcas_casn_meta_outcome η :=
-    hd inhabitant η.(kcas_casn_meta_prophs).
-  #[local] Definition kcas_casn_meta_winner η :=
-    (kcas_casn_meta_outcome η).1.
-  #[local] Definition kcas_casn_meta_success η :=
-    (kcas_casn_meta_outcome η).2.
-  #[local] Definition kcas_casn_meta_final η :=
-    if kcas_casn_meta_success η then §After%V else §Before%V.
-
-  #[local] Instance kcas_casn_meta_eq_dec : EqDecision kcas_casn_meta :=
-    ltac:(solve_decision).
-  #[local] Instance kcas_casn_meta_countable :
-    Countable kcas_casn_meta.
-  Proof.
-    pose encode η := (
-      η.(kcas_casn_meta_descrs),
-      η.(kcas_casn_meta_prophet),
-      η.(kcas_casn_meta_prophs),
-      η.(kcas_casn_meta_undetermined),
-      η.(kcas_casn_meta_post),
-      η.(kcas_casn_meta_lstatus),
-      η.(kcas_casn_meta_witnesses),
-      η.(kcas_casn_meta_waiters),
-      η.(kcas_casn_meta_winning),
-      η.(kcas_casn_meta_owner)
-    ).
-    pose decode := λ '(descrs, prophet, prophs, undetermined, post, lstatus, witnesses, waiters, winning, owner), {|
-      kcas_casn_meta_descrs := descrs ;
-      kcas_casn_meta_prophet := prophet ;
-      kcas_casn_meta_prophs := prophs ;
-      kcas_casn_meta_undetermined := undetermined ;
-      kcas_casn_meta_post := post ;
-      kcas_casn_meta_lstatus := lstatus ;
-      kcas_casn_meta_witnesses := witnesses ;
-      kcas_casn_meta_waiters := waiters ;
-      kcas_casn_meta_winning := winning ;
-      kcas_casn_meta_owner := owner ;
-    |}.
-    refine (inj_countable' encode decode _). intros []. done.
-  Qed.
-
+  #[local] Definition kcas_lstatus_auth' η_lstatus lstatus :=
+    auth_mono_auth _ η_lstatus (DfracOwn 1) lstatus.
   #[local] Definition kcas_lstatus_auth η lstatus :=
-    auth_mono_auth _ η.(kcas_casn_meta_lstatus) (DfracOwn 1) lstatus.
+    kcas_lstatus_auth' η.(kcas_casn_meta_lstatus) lstatus.
   #[local] Definition kcas_lstatus_lb η lstatus :=
     auth_mono_lb _ η.(kcas_casn_meta_lstatus) lstatus.
 
+  #[local] Definition kcas_witness' η_witness :=
+    excl η_witness ().
   #[local] Definition kcas_witness η i : iProp Σ :=
-    ∃ γ_witness,
-    ⌜η.(kcas_casn_meta_witnesses) !! i = Some γ_witness⌝ ∗
-    excl γ_witness ().
+    ∃ η_witness,
+    ⌜η.(kcas_casn_meta_witnesses) !! i = Some η_witness⌝ ∗
+    kcas_witness' η_witness.
 
-  #[local] Definition kcas_waiters η waiters :=
-    ghost_map_auth η.(kcas_casn_meta_waiters) 1 waiters.
-  #[local] Definition kcas_waiter η waiter i :=
+  #[local] Definition kcas_waiters_auth' η_waiters waiters :=
+    ghost_map_auth η_waiters 1 waiters.
+  #[local] Definition kcas_waiters_auth η waiters :=
+    kcas_waiters_auth' η.(kcas_casn_meta_waiters) waiters.
+  #[local] Definition kcas_waiters_elem η waiter i :=
     ghost_map_elem η.(kcas_casn_meta_waiters) waiter (DfracOwn 1) i.
 
+  #[local] Definition kcas_winning' η_winning :=
+    excl η_winning ().
   #[local] Definition kcas_winning η :=
-    excl η.(kcas_casn_meta_winning) ().
+    kcas_winning' η.(kcas_casn_meta_winning).
 
+  #[local] Definition kcas_owner' η_owner :=
+    excl η_owner ().
   #[local] Definition kcas_owner η :=
-    excl η.(kcas_casn_meta_owner) ().
-
-  Inductive kcas_which :=
-    | KcasLoc
-    | KcasCasn.
-
-  Record kcas_param := KcasParam {
-    kcas_param_which : kcas_which ;
-    kcas_param_location : location ;
-    kcas_param_meta : if kcas_param_which then kcas_loc_meta else kcas_casn_meta ;
-  }.
-
-  #[local] Definition kcas_loc_inv_inner' (kcas_inv : kcas_param → iProp Σ) loc γ : iProp Σ :=
-    ∃ casn η i descr,
-    meta casn nroot η ∗
-    ⌜η.(kcas_casn_meta_descrs) !! i = Some descr⌝ ∗
-    ⌜descr.(kcas_descr_loc) = loc⌝ ∗
-    loc ↦ (descr.(kcas_descr_before), descr.(kcas_descr_after), #casn) ∗
-    kcas_lstatus_lb η (KcasUndetermined i) ∗
-    kcas_witness η i ∗
-    kcas_inv (KcasParam KcasCasn casn η).
+    kcas_owner' η.(kcas_casn_meta_owner).
 
   #[local] Definition kcas_au η ι P : iProp Σ :=
     AU <{
@@ -250,30 +341,30 @@ Section kcas_G.
       P
     }>.
 
-  #[local] Definition kcas_waiter_au η ι i Q : iProp Σ :=
-    ∃ descr,
-    ⌜η.(kcas_casn_meta_descrs) !! i = Some descr⌝ ∗
+  #[local] Definition kcas_waiter_au' η ι descr Q : iProp Σ :=
     AU <{
       ∃∃ v,
       kcas_model₁ descr.(kcas_descr_meta) v
     }> @ ⊤ ∖ ↑ι, ∅ <{
-      ⌜v = if kcas_casn_meta_success η then descr.(kcas_descr_after) else descr.(kcas_descr_before)⌝ ∗
+      ⌜v = kcas_descr_final descr η⌝ ∗
       kcas_model₁ descr.(kcas_descr_meta) v
     , COMM
       Q
     }>.
+  #[local] Definition kcas_waiter_au η ι i Q : iProp Σ :=
+    ∃ descr,
+    ⌜η.(kcas_casn_meta_descrs) !! i = Some descr⌝ ∗
+    kcas_waiter_au' η ι descr Q.
 
-  #[local] Definition kcas_casn_inv_inner' (kcas_inv : kcas_param → iProp Σ) casn η ι P : iProp Σ :=
+  #[local] Definition kcas_casn_inv_inner casn η ι P : iProp Σ :=
     ∃ status lstatus waiters,
-    casn.[status] ↦ status ∗
+    casn.[status] ↦ kcas_status_to_val casn η status ∗
     kcas_lstatus_auth η lstatus ∗
-    kcas_waiters η waiters ∗
+    kcas_waiters_auth η waiters ∗
     match lstatus with
-    | KcasUndetermined i =>
-        ⌜i < kcas_casn_meta_size η⌝ ∗
-        ⌜status = ‘Undetermined@η.(kcas_casn_meta_undetermined)( lst_to_val $ kcas_casn_meta_cass casn η )%V⌝ ∗
+    | KcasRunning i =>
+        ⌜status = KcasUndetermined⌝ ∗
         ( [∗ list] descr ∈ take i η.(kcas_casn_meta_descrs),
-          meta descr.(kcas_descr_loc) nroot descr.(kcas_descr_meta) ∗
           kcas_model₂ descr.(kcas_descr_meta) descr.(kcas_descr_before)
         ) ∗
         ( [∗ list] j ∈ seq 0 (kcas_casn_meta_size η - i),
@@ -293,10 +384,8 @@ Section kcas_G.
         ∃ prophs,
         ⌜status = kcas_casn_meta_final η⌝ ∗
         ( [∗ list] i ↦ descr ∈ η.(kcas_casn_meta_descrs),
-          meta descr.(kcas_descr_loc) nroot descr.(kcas_descr_meta) ∗
-          ( kcas_model₂ descr.(kcas_descr_meta) (if kcas_casn_meta_success η then descr.(kcas_descr_after) else descr.(kcas_descr_before))
+            kcas_model₂ descr.(kcas_descr_meta) (kcas_descr_final descr η)
           ∨ kcas_witness η i
-          )
         ) ∗
         ( [∗ map] waiter ↦ i ∈ waiters,
           ∃ Q,
@@ -308,147 +397,739 @@ Section kcas_G.
         identifier_model (kcas_casn_meta_winner η) ∗
         (kcas_owner η ∨ P)
     end.
-
-  #[local] Definition kcas_inv_pre ι
-  : (kcas_param -d> iProp Σ) →
-    kcas_param -d> iProp Σ
+  #[local] Definition kcas_casn_inv_pre ι
+    (kcas_casn_inv' : location * kcas_casn_meta * option nat -d> iProp Σ)
+    (kcas_loc_inv' : location -d> iProp Σ)
+  : location * kcas_casn_meta * option nat -d> iProp Σ
   :=
-    λ kcas_inv param,
-      match param.(kcas_param_which) as which
-      return (if which then kcas_loc_meta else kcas_casn_meta) → _
-      with
-      | KcasLoc => λ γ,
-          let loc := param.(kcas_param_location) in
-          inv (ι.@"loc") (kcas_loc_inv_inner' kcas_inv loc γ)
-      | KcasCasn => λ η,
-          let casn := param.(kcas_param_location) in
-          ∃ P,
-          casn.[proph] ↦□ #η.(kcas_casn_meta_prophet) ∗
-          saved_prop η.(kcas_casn_meta_post) P ∗
-          inv (ι.@"casn".@casn) (kcas_casn_inv_inner' kcas_inv casn η ι P)
-      end%I
-      param.(kcas_param_meta).
-  #[local] Instance kcas_inv_pre_contractive ι :
-    Contractive (kcas_inv_pre ι).
+    λ '(casn, η, i), (
+      ∃ P,
+      casn.[proph] ↦□ #η.(kcas_casn_meta_prophet) ∗
+      saved_prop η.(kcas_casn_meta_post) P ∗
+      ⌜NoDup (kcas_descr_loc <$> η.(kcas_casn_meta_descrs))⌝ ∗
+      inv (ι.@"casn") (kcas_casn_inv_inner casn η ι P) ∗
+      ( if i is Some i then
+          [∗ list] j ↦ descr ∈ η.(kcas_casn_meta_descrs),
+          if decide (j = i) then
+            meta descr.(kcas_descr_loc) nroot descr.(kcas_descr_meta)
+          else
+            meta descr.(kcas_descr_loc) nroot descr.(kcas_descr_meta) ∗
+            kcas_loc_inv' descr.(kcas_descr_loc)
+        else
+          [∗ list] descr ∈ η.(kcas_casn_meta_descrs),
+          meta descr.(kcas_descr_loc) nroot descr.(kcas_descr_meta) ∗
+          kcas_loc_inv' descr.(kcas_descr_loc)
+      )
+    )%I.
+  #[local] Instance kcas_casn_inv_pre_contractive ι n :
+    Proper (dist_later n ==> (≡{n}≡) ==> (≡{n}≡)) (kcas_casn_inv_pre ι).
   Proof.
-    rewrite /kcas_inv_pre /kcas_loc_inv_inner' /kcas_casn_inv_inner' => n Ψ1 Ψ2 HΨ param.
-    destruct param as ([], ?, ?); solve_contractive.
+    solve_proper.
   Qed.
-  #[local] Definition kcas_inv ι : kcas_param → iProp Σ :=
-    fixpoint (kcas_inv_pre ι).
 
-  #[local] Definition kcas_loc_inv_inner loc γ ι :=
-    kcas_loc_inv_inner' (kcas_inv ι) loc γ.
-  #[local] Definition kcas_loc_inv' loc γ ι :=
-    kcas_inv ι (KcasParam KcasLoc loc γ).
-  Definition kcas_loc_inv loc ι : iProp Σ :=
-    ∃ γ,
-    meta loc nroot γ ∗
-    kcas_loc_inv' loc γ ι.
+  #[local] Definition kcas_loc_inv_inner'' full kcas_casn_inv' loc : iProp Σ :=
+    ∃ casn η i descr,
+    meta casn nroot η ∗
+    ⌜η.(kcas_casn_meta_descrs) !! i = Some descr⌝ ∗
+    ⌜loc = descr.(kcas_descr_loc)⌝ ∗
+    loc ↦ᵣ kcas_state casn descr ∗
+    kcas_lstatus_lb η (KcasRunning (S i)) ∗
+    kcas_witness η i ∗
+    kcas_casn_inv' (casn, η, if full then None else Some i).
+  #[local] Definition kcas_loc_inv_inner' :=
+    kcas_loc_inv_inner'' false.
+  #[local] Definition kcas_loc_inv_pre ι
+    (kcas_casn_inv' : location * kcas_casn_meta * option nat -d> iProp Σ)
+    (kcas_loc_inv' : location -d> iProp Σ)
+  : location -d> iProp Σ
+  :=
+    λ loc,
+      inv (ι.@"loc") (kcas_loc_inv_inner' kcas_casn_inv' loc).
+  #[local] Instance kcas_loc_inv_pre_contractive ι n :
+    Proper (dist_later n ==> dist_later n ==> (≡{n}≡)) (kcas_loc_inv_pre ι).
+  Proof.
+    rewrite /kcas_loc_inv_pre /kcas_loc_inv_inner' /kcas_loc_inv_inner'' /curry.
+    solve_contractive.
+  Qed.
 
-  #[local] Definition kcas_casn_inv_inner casn η ι P :=
-    kcas_casn_inv_inner' (kcas_inv ι) casn η ι P.
-  #[local] Definition kcas_casn_inv' casn η ι :=
-    kcas_inv ι (KcasParam KcasCasn casn η).
+  #[local] Definition kcas_casn_inv'' ι :=
+    fixpoint_A (kcas_casn_inv_pre ι) (kcas_loc_inv_pre ι).
+  #[local] Definition kcas_casn_inv' ι casn η :=
+    kcas_casn_inv'' ι (casn, η, None).
   #[local] Definition kcas_casn_inv casn ι : iProp Σ :=
     ∃ η,
     meta casn nroot η ∗
-    kcas_casn_inv' casn η ι.
+    kcas_casn_inv' ι casn η.
+
+  #[local] Definition kcas_loc_inv' ι :=
+    fixpoint_B (kcas_casn_inv_pre ι) (kcas_loc_inv_pre ι).
+  #[local] Definition kcas_loc_inv_inner loc ι : iProp Σ :=
+    kcas_loc_inv_inner'' true (kcas_casn_inv'' ι) loc.
+  Definition kcas_loc_inv loc ι : iProp Σ :=
+    ∃ γ,
+    meta loc nroot γ ∗
+    kcas_loc_inv' ι loc.
 
   Definition kcas_loc_model loc v : iProp Σ :=
     ∃ γ,
     meta loc nroot γ ∗
     kcas_model₁ γ v.
 
-  #[local] Instance kcas_inv_persistent ι param :
-    Persistent (kcas_inv ι param).
+  #[local] Lemma kcas_casn_inv'_unfold ι casn η :
+    kcas_casn_inv' ι casn η ⊣⊢
+    kcas_casn_inv_pre ι (kcas_casn_inv'' ι) (kcas_loc_inv' ι) (casn, η, None).
   Proof.
-    rewrite /kcas_inv.
-    apply fixpoint_ind.
-  Admitted.
+    symmetry. apply (fixpoint_A_unfold (kcas_casn_inv_pre ι) (kcas_loc_inv_pre ι) _).
+  Qed.
 
-  #[local] Lemma kcas_finish_spec_loser id casn η ι status :
+  #[local] Lemma kcas_loc_inv'_unfold loc ι :
+    kcas_loc_inv' ι loc ⊣⊢
+    inv (ι.@"loc") (kcas_loc_inv_inner' (kcas_casn_inv'' ι) loc).
+  Proof.
+    symmetry. apply (fixpoint_B_unfold (kcas_casn_inv_pre ι) (kcas_loc_inv_pre ι) _).
+  Qed.
+  #[local] Lemma kcas_loc_inv'_intro loc ι :
+    inv (ι.@"loc") (kcas_loc_inv_inner' (kcas_casn_inv'' ι) loc) ⊢
+    kcas_loc_inv' ι loc.
+  Proof.
+    setoid_rewrite <- (fixpoint_B_unfold (kcas_casn_inv_pre ι) (kcas_loc_inv_pre ι) _).
+    iIntros "#Hloc_inv".
+    iApply (inv_alter with "Hloc_inv"). iIntros "!> !> (%casn & %η & %i & %descr & Hcasn_meta & %Hdescrs_lookup & -> & Hloc & Hlstatus_lb & Hwitness & Hcasn_inv')".
+    iFrame. iSteps.
+  Qed.
+  #[local] Lemma kcas_loc_inv'_elim loc γ ι :
+    meta loc nroot γ -∗
+    kcas_loc_inv' ι loc -∗
+    inv (ι.@"loc") (kcas_loc_inv_inner loc ι).
+  Proof.
+    setoid_rewrite <- (fixpoint_B_unfold (kcas_casn_inv_pre ι) (kcas_loc_inv_pre ι) _).
+    iIntros "#Hloc_meta #Hloc_inv".
+    iApply (inv_alter with "Hloc_inv"). iIntros "!> !> (%casn & %η & %i & %descr & Hcasn_meta & %Hdescrs_lookup & -> & Hloc & Hlstatus_lb & Hwitness & Hcasn_inv')".
+    iSplitL.
+    - iFrame. iSteps.
+      setoid_rewrite <- (fixpoint_A_unfold (kcas_casn_inv_pre ι) (kcas_loc_inv_pre ι) _).
+      iDestruct "Hcasn_inv'" as "(%P & Hcasn_proph & Hpost & %Hlocs & Hcasn_inv & Hlocs_inv)".
+      iSteps.
+      iApply (big_sepL_impl with "Hlocs_inv"). iIntros "!> %i' %descr' %Hdescr_lookup' H".
+      case_decide; last iSteps.
+      simplify.
+      iDestruct (meta_agree with "Hloc_meta H") as %->.
+      setoid_rewrite <- (fixpoint_B_unfold (kcas_casn_inv_pre ι) (kcas_loc_inv_pre ι) _).
+      iSteps.
+    - iSteps.
+      setoid_rewrite <- (fixpoint_A_unfold (kcas_casn_inv_pre ι) (kcas_loc_inv_pre ι) _).
+      iSteps.
+      iApply (big_sepL_impl with "[$]").
+      iSteps.
+      case_decide; iSteps.
+  Qed.
+
+  #[global] Instance kcas_loc_model_persistent loc ι :
+    Timeless (kcas_loc_model loc ι).
+  Proof.
+    apply _.
+  Qed.
+  #[local] Instance kcas_casn_inv'_persistent casn η ι :
+    Persistent (kcas_casn_inv' ι casn η).
+  Proof.
+    rewrite kcas_casn_inv'_unfold /kcas_casn_inv_pre.
+    setoid_rewrite kcas_loc_inv'_unfold.
+    apply _.
+  Qed.
+  #[local] Instance kcas_loc_inv'_persistent loc ι :
+    Persistent (kcas_loc_inv' ι loc).
+  Proof.
+    rewrite kcas_loc_inv'_unfold.
+    apply _.
+  Qed.
+  #[global] Instance kcas_loc_inv_persistent loc ι :
+    Persistent (kcas_loc_inv loc ι).
+  Proof.
+    rewrite /kcas_loc_inv.
+    apply _.
+  Qed.
+
+  #[local] Lemma kcas_model_alloc v :
+    ⊢ |==>
+      ∃ γ,
+      kcas_model₁ γ v ∗
+      kcas_model₂ γ v.
+  Proof.
+    apply twins_alloc'.
+  Qed.
+  #[local] Lemma kcas_model_agree γ v1 v2 :
+    kcas_model₁ γ v1 -∗
+    kcas_model₂ γ v2 -∗
+    ⌜v1 = v2⌝.
+  Proof.
+    apply: twins_agree_L.
+  Qed.
+  #[local] Lemma kcas_model₂_exclusive γ v1 v2 :
+    kcas_model₂ γ v1 -∗
+    kcas_model₂ γ v2 -∗
+    False.
+  Proof.
+    apply twins_twin2_exclusive.
+  Qed.
+
+  #[local] Lemma kcas_lstatus_alloc lstatus :
+    ⊢ |==>
+      ∃ η_lstatus,
+      kcas_lstatus_auth' η_lstatus lstatus.
+  Proof.
+    apply: auth_mono_alloc.
+  Qed.
+  #[local] Lemma kcas_lstatus_lb_get η lstatus :
+    kcas_lstatus_auth η lstatus ⊢
+    kcas_lstatus_lb η lstatus.
+  Proof.
+    apply auth_mono_lb_get.
+  Qed.
+  #[local] Lemma kcas_lstatus_lb_get_running0 η lstatus :
+    kcas_lstatus_auth η lstatus ⊢
+    kcas_lstatus_lb η (KcasRunning 0).
+  Proof.
+    apply auth_mono_lb_get_mono, kcas_lsteps_running0.
+  Qed.
+  #[local] Lemma kcas_lstatus_lb_get_finished {η} lstatus :
+    kcas_lstatus_auth η KcasFinished ⊢
+    kcas_lstatus_lb η lstatus.
+  Proof.
+    destruct lstatus.
+    - apply auth_mono_lb_get_mono'. done.
+    - apply kcas_lstatus_lb_get.
+  Qed.
+  #[local] Lemma kcas_lstatus_finished η lstatus :
+    kcas_lstatus_auth η lstatus -∗
+    kcas_lstatus_lb η KcasFinished -∗
+    ⌜lstatus = KcasFinished⌝.
+  Proof.
+    iIntros "Hlstatus_auth Hlstatus_lb".
+    iDestruct (auth_mono_lb_valid with "Hlstatus_auth Hlstatus_lb") as %->%kcas_lsteps_finished.
+    iSteps.
+  Qed.
+  #[local] Lemma kcas_lstatus_le η i1 i2 :
+    kcas_lstatus_auth η (KcasRunning i1) -∗
+    kcas_lstatus_lb η (KcasRunning i2) -∗
+    ⌜i2 ≤ i1⌝.
+  Proof.
+    iIntros "Hlstatus_auth Hlstatus_lb".
+    iDestruct (auth_mono_lb_valid with "Hlstatus_auth Hlstatus_lb") as %Hlsteps.
+    iPureIntro. eapply kcas_lsteps_le; done.
+  Qed.
+  #[local] Lemma kcas_lstatus_update {η lstatus} lstatus' :
+    kcas_lstep lstatus lstatus' →
+    kcas_lstatus_auth η lstatus ⊢ |==>
+    kcas_lstatus_auth η lstatus'.
+  Proof.
+    apply auth_mono_update'.
+  Qed.
+
+  #[local] Lemma kcas_witness_alloc :
+    ⊢ |==>
+      ∃ η_witness,
+      kcas_witness' η_witness.
+  Proof.
+    apply excl_alloc.
+  Qed.
+  #[local] Lemma kcas_witness_exclusive η i :
+    kcas_witness η i -∗
+    kcas_witness η i -∗
+    False.
+  Proof.
+    iIntros "(%γ_witness & %Hlookup & Hexcl1) (%_γ_witness & %_Hlookup & Hexcl2)".
+    simplify.
+    iApply (excl_exclusive with "Hexcl1 Hexcl2").
+  Qed.
+
+  #[local] Lemma kcas_waiters_alloc :
+    ⊢ |==>
+      ∃ η_waiters,
+      kcas_waiters_auth' η_waiters ∅.
+  Proof.
+    apply ghost_map_alloc_empty.
+  Qed.
+  #[local] Lemma kcas_waiters_insert {η waiters} i P :
+    kcas_waiters_auth η waiters ⊢ |==>
+      ∃ waiter,
+      kcas_waiters_auth η (<[waiter := i]> waiters) ∗
+      kcas_waiters_elem η waiter i ∗
+      saved_prop waiter P.
+  Proof.
+    iIntros "Hwaiters_auth".
+    iMod (saved_prop_alloc_cofinite (dom waiters)) as "(%waiter & %Hwaiter & #Hwaiter)".
+    iMod (ghost_map_insert with "Hwaiters_auth") as "(Hwaiters_auth & Hwaiters_elem)".
+    { apply not_elem_of_dom. done. }
+    iSteps.
+  Qed.
+  #[local] Lemma kcas_waiters_lookup η waiters waiter i :
+    kcas_waiters_auth η waiters -∗
+    kcas_waiters_elem η waiter i -∗
+    ⌜waiters !! waiter = Some i⌝.
+  Proof.
+    apply ghost_map_lookup.
+  Qed.
+  #[local] Lemma kcas_waiters_delete η waiters waiter i :
+    kcas_waiters_auth η waiters -∗
+    kcas_waiters_elem η waiter i ==∗
+    kcas_waiters_auth η (delete waiter waiters).
+  Proof.
+    apply ghost_map_delete.
+  Qed.
+
+  #[local] Lemma kcas_winning_alloc :
+    ⊢ |==>
+      ∃ η_winning,
+      kcas_winning' η_winning.
+  Proof.
+    apply excl_alloc.
+  Qed.
+  #[local] Lemma kcas_winning_exclusive η :
+    kcas_winning η -∗
+    kcas_winning η -∗
+    False.
+  Proof.
+    apply excl_exclusive.
+  Qed.
+
+  #[local] Lemma kcas_owner_alloc :
+    ⊢ |==>
+      ∃ η_owner,
+      kcas_owner' η_owner.
+  Proof.
+    apply excl_alloc.
+  Qed.
+  #[local] Lemma kcas_owner_exclusive η :
+    kcas_owner η -∗
+    kcas_owner η -∗
+    False.
+  Proof.
+    apply excl_exclusive.
+  Qed.
+
+  #[local] Lemma kcas_casn_wait {casn η ι P i} descr γ Q :
+    η.(kcas_casn_meta_descrs) !! i = Some descr →
+    descr.(kcas_descr_meta) = γ →
+    inv (ι.@"casn") (kcas_casn_inv_inner casn η ι P) -∗
+    kcas_witness η i -∗
+    kcas_waiter_au' η ι descr Q -∗
+      |={⊤ ∖ ↑ι.@"loc"}=>
+      ∃ waiter,
+      kcas_witness η i ∗
+      saved_prop waiter Q ∗
+      kcas_waiters_elem η waiter i.
+  Proof.
+    iIntros (Hdescrs_lookup <-) "#Hcasn_inv Hwitness H".
+    iInv "Hcasn_inv" as "(%status & %lstatus & %waiters & Hcasn_status & Hlstatus_auth & >Hwaiters_auth & Hlstatus)".
+    iMod (kcas_waiters_insert i Q with "Hwaiters_auth") as "(%waiter & Hwaiters_auth & Hwaiters_elem & #Hwaiter)".
+    destruct lstatus as [j |].
+
+    - iDestruct "Hlstatus" as "(>-> & Hmodels & Hwitnesses & Hwaiters & Hproph & Hau)".
+      iDestruct (big_sepM_insert_2 _ _ waiter i with "[H] Hwaiters") as "Hwaiters"; first iSteps.
+      iSplitR "Hwitness Hwaiters_elem". { do 2 iFrame. iSteps. }
+      iModIntro.
+
+      iFrame. iSteps.
+
+    - iDestruct "Hlstatus" as "(%prophs & >-> & >Hmodels & Hwaiters & Hproph & Hwinning & Hwinner & HP)".
+      iDestruct (big_sepL_lookup_acc with "Hmodels") as "([Hmodel₂ | _Hwitness] & Hmodels)"; first done; last first.
+      { iDestruct (kcas_witness_exclusive with "Hwitness _Hwitness") as %[]. }
+      iApply (fupd_mask_mono (⊤ ∖ ↑ι)); first solve_ndisj.
+      iMod "H" as "(%v & Hmodel₁ & _ & H)".
+      iDestruct (kcas_model_agree with "Hmodel₁ Hmodel₂") as %->.
+      iMod ("H" with "[$Hmodel₁ //]") as "HQ".
+      iDestruct ("Hmodels" with "[Hmodel₂]") as "Hmodels"; first iSteps.
+      iDestruct (big_sepM_insert_2 _ _ waiter i with "[HQ] Hwaiters") as "Hwaiters"; first iSteps.
+      iSplitR "Hwitness Hwaiters_elem". { do 2 iFrame. iSteps. }
+      iModIntro.
+
+      iFrame. iSteps.
+  Qed.
+  #[local] Lemma kcas_casn_retrieve casn η ι P waiter Q i :
+    inv (ι.@"casn") (kcas_casn_inv_inner casn η ι P) -∗
+    kcas_lstatus_lb η KcasFinished -∗
+    saved_prop waiter Q -∗
+    kcas_waiters_elem η waiter i ={⊤}=∗
+    ▷^2 Q.
+  Proof.
+    iIntros "#Hcasn_inv #Hlstatus_lb #Hwaiter Hwaiters_elem".
+    iInv "Hcasn_inv" as "(%status & %lstatus & %waiters & Hcasn_status & >Hlstatus_auth & >Hwaiters_auth & Hlstatus)".
+    iDestruct (kcas_lstatus_finished with "Hlstatus_auth Hlstatus_lb") as %->.
+    iDestruct "Hlstatus" as "(%prophs & >-> & Hmodels & Hwaiters & Hproph & Hwinning & Hwinner & HP)".
+    iDestruct (kcas_waiters_lookup with "Hwaiters_auth Hwaiters_elem") as %Hwaiters_lookup.
+    iMod (kcas_waiters_delete with "Hwaiters_auth Hwaiters_elem") as "Hwaiters_auth".
+    iDestruct (big_sepM_delete with "Hwaiters") as "((%_Q & _Hwaiter & HQ) & Hwaiters)"; first done.
+    iDestruct (saved_prop_agree with "Hwaiter _Hwaiter") as "Heq".
+    iSplitR "HQ Heq". { do 2 iFrame. iSteps. }
+    iModIntro.
+
+    do 3 iModIntro. iRewrite "Heq". iSteps.
+  Qed.
+
+  #[local] Lemma kcas_finish_spec_loser gid casn η ι (status : val) :
     status = §Before%V ∨ status = §After%V →
-    id ≠ kcas_casn_meta_winner η →
+    gid ≠ kcas_casn_meta_winner η →
     {{{
-      kcas_casn_inv' casn η ι
+      meta casn nroot η ∗
+      kcas_casn_inv' ι casn η
     }}}
-      kcas_finish #id #casn status
+      kcas_finish #gid #casn status
     {{{
       RET #(kcas_casn_meta_success η);
       kcas_lstatus_lb η KcasFinished
     }}}.
   Proof.
   Admitted.
-  #[local] Lemma kcas_finish_spec_winner_after id casn η ι :
-    id = kcas_casn_meta_winner η →
+  #[local] Lemma kcas_finish_spec_winner_after gid casn η ι :
+    gid = kcas_casn_meta_winner η →
     {{{
-      kcas_casn_inv' casn η ι ∗
-      identifier_model id ∗
-      kcas_lstatus_lb η (KcasUndetermined (kcas_casn_meta_size η - 1))
+      meta casn nroot η ∗
+      kcas_casn_inv' ι casn η ∗
+      identifier_model gid ∗
+      kcas_lstatus_lb η (KcasRunning (kcas_casn_meta_size η - 1))
     }}}
-      kcas_finish #id #casn §After
+      kcas_finish #gid #casn §After
     {{{
       RET #(kcas_casn_meta_success η);
       kcas_lstatus_lb η KcasFinished
     }}}.
   Proof.
   Admitted.
-  #[local] Lemma kcas_finish_spec_winner_before id casn η ι :
-    id = kcas_casn_meta_winner η →
+  #[local] Lemma kcas_finish_spec_winner_before gid casn η ι P :
+    gid = kcas_casn_meta_winner η →
     {{{
-      kcas_casn_inv' casn η ι ∗
-      kcas_winning η
+      meta casn nroot η ∗
+      kcas_casn_inv' ι casn η ∗
+      kcas_winning η ∗
+      saved_prop η.(kcas_casn_meta_post) P ∗
+      P
     }}}
-      kcas_finish #id #casn §Before
+      kcas_finish #gid #casn §Before
     {{{
-      RET #false;
+      RET #(kcas_casn_meta_success η);
+      kcas_lstatus_lb η KcasFinished
+    }}}.
+  Proof.
+  Admitted.
+  #[local] Lemma kcas_finish_spec_after gid casn η ι i :
+    kcas_casn_meta_size η - 1 ≤ i →
+    {{{
+      meta casn nroot η ∗
+      kcas_casn_inv' ι casn η ∗
+      kcas_lstatus_lb η (KcasRunning i)
+    }}}
+      kcas_finish #gid #casn §After
+    {{{
+      RET #(kcas_casn_meta_success η);
       kcas_lstatus_lb η KcasFinished
     }}}.
   Proof.
   Admitted.
 
-  #[local] Definition kcas_determine_specification : iProp Σ :=
-    ∀ casn η ι,
-    {{{
-      kcas_casn_inv' casn η ι
-    }}}
-      kcas_determine #casn
-    {{{
-      RET #(kcas_casn_meta_success η);
-      kcas_lstatus_lb η KcasFinished
-    }}}.
+  #[local] Lemma kcas_determine_as_get_as_determine_spec ι :
+    ⊢ (
+      ∀ casn η cass i,
+      {{{
+        ⌜cass = lst_to_val (drop i (kcas_casn_meta_cass casn η))⌝ ∗
+        meta casn nroot η ∗
+        kcas_casn_inv' ι casn η ∗
+        kcas_lstatus_lb η (KcasRunning i)
+      }}}
+        kcas_determine_as #casn cass
+      {{{
+        RET #(kcas_casn_meta_success η);
+        kcas_lstatus_lb η KcasFinished
+      }}}
+    ) ∧ (
+      ∀ state casn η descr,
+      {{{
+        ⌜state = kcas_state casn descr⌝ ∗
+        ⌜descr ∈ η.(kcas_casn_meta_descrs)⌝ ∗
+        meta casn nroot η ∗
+        kcas_casn_inv' ι casn η
+      }}}
+        kcas_get_as state
+      {{{
+        RET kcas_descr_final descr η;
+        kcas_lstatus_lb η KcasFinished ∗
+        £ 1
+      }}}
+    ) ∧ (
+      ∀ casn η,
+      {{{
+        meta casn nroot η ∗
+        kcas_casn_inv' ι casn η
+      }}}
+        kcas_determine #casn
+      {{{
+        RET #(kcas_casn_meta_success η);
+        kcas_lstatus_lb η KcasFinished
+      }}}
+    ).
+  Proof.
+    iLöb as "HLöb".
+    iDestruct "HLöb" as "(Hdetermine_as & Hget_as & Hdetermine)".
+    repeat iSplit.
 
-  #[local] Lemma kcas_determine_aux_spec {casn η ι cass} i :
+    { iIntros "%casn %η %cass %i !> %Φ (-> & #Hcasn_meta & #Hcasn_inv' & #Hlstatus_lb) HΦ".
+      iDestruct (kcas_casn_inv'_unfold with "Hcasn_inv'") as "(%P & #Hcasn_proph & #Hpost & %Hlocs & #Hcasn_inv & #Hlocs_inv)".
+
+      wp_recs credit:"H£".
+      wp_smart_apply (wp_id with "[//]") as (gid) "Hgid".
+
+      destruct (η.(kcas_casn_meta_descrs) !! i) as [descr |] eqn:Hdescrs_lookup.
+
+      - apply lookup_lt_Some in Hdescrs_lookup as Hi.
+        erewrite drop_S; last first.
+        { apply list_lookup_fmap_Some. naive_solver. }
+        iDestruct (big_sepL_lookup with "Hlocs_inv") as "(Hloc_meta & Hloc_inv')"; first done.
+        iDestruct (kcas_loc_inv'_elim with "Hloc_meta Hloc_inv'") as "Hloc_inv".
+        wp_pures.
+
+        wp_bind (!_)%E.
+        iInv "Hloc_inv" as "(%casn' & %η' & %i' & %descr' & #Hcasn'_meta & >%Hdescrs'_lookup & >%Hloc' & Hloc & #Hlstatus'_lb & Hwitness' & #Hcasn'_inv')".
+        wp_load.
+        iDestruct (kcas_casn_inv'_unfold with "Hcasn'_inv'") as "(%P' & #Hcasn'_proph & #Hpost' & %Hlocs' & #Hcasn'_inv & #Hlocs'_inv)".
+        iAssert ⌜descr'.(kcas_descr_meta) = descr.(kcas_descr_meta)⌝%I as %Hmeta'.
+        { iDestruct (big_sepL_lookup with "Hlocs_inv") as "(Hloc_meta_1 & _)"; first done.
+          iDestruct (big_sepL_lookup with "Hlocs'_inv") as "(Hloc_meta_2 & _)"; first done.
+          iEval (rewrite -Hloc') in "Hloc_meta_2".
+          iApply (meta_agree with "Hloc_meta_2 Hloc_meta_1").
+        }
+        destruct (decide (casn' = casn)) as [-> | Hcasn'].
+
+        + iDestruct (meta_agree with "Hcasn_meta Hcasn'_meta") as %<-. iClear "Hcasn'_meta".
+          assert (i' = i) as ->.
+          { eapply NoDup_lookup; first done.
+            - rewrite list_lookup_fmap Hdescrs'_lookup //.
+            - rewrite list_lookup_fmap Hdescrs_lookup -Hloc' //.
+          }
+          simplify.
+          iSplitR "HΦ". { iFrame. iSteps. }
+          iModIntro. clear.
+
+          wp_equal as ? | _; first naive_solver.
+          wp_smart_apply ("Hdetermine_as" with "[$Hcasn_meta $Hcasn_inv' $Hlstatus'_lb //] HΦ").
+
+        + destruct (decide (gid = kcas_casn_meta_winner η ∧ descr.(kcas_descr_before) ≠ kcas_descr_final descr' η')) as [(-> & Hfail) | Hok%not_and_r_alt].
+
+          * iInv "Hcasn_inv" as "(%status & %lstatus & %waiters & Hcasn_status & Hlstatus_auth & Hwaiters_auth & Hlstatus)".
+            destruct lstatus as [j |]; last first.
+            { iDestruct "Hlstatus" as "(%prophs & _ & _ & _ & _ & _ & >_Hgid & _)".
+              iDestruct (identifier_model_exclusive with "Hgid _Hgid") as %[].
+            }
+            iDestruct "Hlstatus" as "(>-> & Hmodels & Hwitnesses & Hwaiters & Hproph & [(Hau & Hwinning) | >_Hgid])"; last first.
+            { iDestruct (identifier_model_exclusive with "Hgid _Hgid") as %[]. }
+            iMod (lc_fupd_elim_later with "H£ Hau") as "Hau".
+            iSplitR "Hloc Hwitness' Hau Hwinning HΦ". { do 2 iFrame. iSteps. }
+            iModIntro. clear j waiters.
+
+            iMod (kcas_casn_wait _ _ P with "Hcasn'_inv Hwitness' [Hau]") as "(%waiter & Hwitness' & #Hwaiter & Hwaiters'_elem)"; [solve_ndisj | done.. | |].
+            { admit.
+            }
+
+            iSplitR "Hwinning Hwaiters'_elem HΦ". { do 2 iFrame. iSteps. }
+            iModIntro.
+
+            wp_equal as _ | ?; last naive_solver.
+
+            iClear "Hlstatus'_lb".
+            wp_smart_apply ("Hget_as" with "[$Hcasn'_meta $Hcasn'_inv']") as "(#Hlstatus'_lb & H£)".
+            { iSteps. iPureIntro. eapply elem_of_list_lookup_2. done. }
+            iMod (kcas_casn_retrieve with "Hcasn'_inv Hlstatus'_lb Hwaiter Hwaiters'_elem") as "HP".
+
+            wp_smart_apply wp_equal.
+            rewrite bool_decide_eq_false_2 //.
+            wp_smart_apply (kcas_finish_spec_winner_before with "[$Hcasn_meta $Hcasn_inv' $Hwinning $Hpost $HP] HΦ"); first done.
+
+          * iSplitR "Hgid HΦ". { iFrame. iSteps. }
+            iModIntro.
+
+            wp_equal as _ | ?; last naive_solver.
+
+            iClear "Hlstatus'_lb".
+            wp_smart_apply ("Hget_as" with "[$Hcasn'_meta $Hcasn'_inv']") as "(#Hlstatus'_lb & H£)".
+            { iSteps. iPureIntro. eapply elem_of_list_lookup_2. done. }
+
+            wp_smart_apply wp_equal.
+            destruct Hok as [(Hgid & Hfail) | Hok%dec_stable].
+
+            -- rewrite bool_decide_eq_false_2 //.
+               wp_smart_apply (kcas_finish_spec_loser with "[$Hcasn_meta $Hcasn_inv'] HΦ"); auto.
+
+            -- rewrite bool_decide_eq_true_2 //.
+               wp_pures.
+
+               wp_bind (_.{status})%E.
+               iInv "Hcasn_inv" as "(%status & %lstatus & %waiters & Hcasn_status & Hlstatus_auth & Hwaiters_auth & Hlstatus)".
+               wp_load.
+               destruct lstatus as [j |].
+
+               ++ iDestruct "Hlstatus" as "(-> & Hlstatus)".
+                  iSplitR "HΦ". { do 2 iFrame. iSteps. }
+                  iModIntro. clear waiters j.
+
+                  wp_pures.
+
+                  wp_bind (CAS _ _ _).
+                  iInv "Hloc_inv" as "(%casn'' & %η'' & %i'' & %descr'' & #Hcasn''_meta & >%Hdescrs''_lookup & >%Hloc'' & Hloc & #Hlstatus''_lb & Hwitness'' & #Hcasn''_inv')".
+                  wp_cas as _ | (_ & _ & [= -> _ _]).
+
+                  ** iSplitR "HΦ". { iFrame. iSteps. }
+                     iModIntro.
+
+                     wp_smart_apply ("Hdetermine_as" with "[$Hcasn_meta $Hcasn_inv' $Hlstatus_lb] HΦ").
+                     { iPureIntro.
+                       erewrite (drop_S _ _ i); first done.
+                       rewrite list_lookup_fmap Hdescrs_lookup //.
+                    }
+
+                  ** iDestruct (meta_agree with "Hcasn'_meta Hcasn''_meta") as %<-. iClear "Hcasn''_meta Hcasn''_inv' Hlstatus''_lb".
+                     assert (i'' = i') as ->.
+                     { eapply NoDup_lookup; first done.
+                       - rewrite list_lookup_fmap Hdescrs''_lookup //.
+                       - rewrite list_lookup_fmap Hdescrs'_lookup /=. congruence.
+                     }
+                     simplify.
+
+                     iInv "Hcasn'_inv" as "(%status' & %lstatus' & %waiters' & Hcasn'_status & >Hlstatus'_auth & Hwaiters'_auth & Hlstatus')".
+                     iDestruct (kcas_lstatus_finished with "Hlstatus'_auth Hlstatus'_lb") as %->.
+                     iDestruct "Hlstatus'" as "(%prophs' & >-> & Hmodels' & Hwaiters' & Hproph' & Hwinning' & Hwinner' & HP')".
+                     iDestruct (big_sepL_lookup_acc with "Hmodels'") as "([>Hmodel₂ | >Hwitness'] & Hmodels')"; first done; last first.
+                     { iDestruct (kcas_witness_exclusive with "Hwitness'' Hwitness'") as %[]. }
+
+                     iDestruct ("Hmodels'" with "[$Hwitness'']") as "Hmodels'".
+                     iSplitR "Hloc Hmodel₂ HΦ". { do 2 iFrame. iSteps. }
+                     iModIntro. clear waiters' prophs'.
+
+                     iEval (rewrite Hmeta') in "Hmodel₂".
+                     iInv "Hcasn_inv" as "(%status & %lstatus & %waiters & Hcasn_status & >Hlstatus_auth & Hwaiters_auth & Hlstatus)".
+                     destruct lstatus as [j |]; last first.
+                     { iDestruct "Hlstatus" as "(%prophs & >-> & Hmodels & Hwaiters & Hproph & Hwinning & Hwinner & HP)".
+                       admit.
+                     }
+                     iDestruct "Hlstatus" as "(>-> & >Hmodels & >Hwitnesses & Hwaiters & Hproph & HP)".
+                     iAssert ⌜j = i⌝%I as %->.
+                     { destruct (Nat.lt_trichotomy j i) as [? | [-> | ?]].
+                       - iDestruct (kcas_lstatus_le with "Hlstatus_auth Hlstatus_lb") as %?. lia.
+                       - iSteps.
+                       - iDestruct (big_sepL_lookup with "Hmodels") as "_Hmodel₂".
+                         { apply lookup_take_Some. done. }
+                         iDestruct (kcas_model₂_exclusive with "Hmodel₂ _Hmodel₂") as %[].
+                     }
+                     iMod (kcas_lstatus_update (KcasRunning (S i)) with "Hlstatus_auth") as "Hlstatus_auth"; first done.
+                     iClear "Hlstatus_lb". iDestruct (kcas_lstatus_lb_get with "Hlstatus_auth") as "#Hlstatus_lb".
+                     iEval (rewrite -Hok) in "Hmodel₂".
+                     iDestruct (big_sepL_snoc_2 with "Hmodels Hmodel₂") as "Hmodels"; first done.
+                     iEval (rewrite -take_S_r //) in "Hmodels".
+                     rewrite -(Nat.succ_pred_pos (kcas_casn_meta_size η - i)).
+                     { rewrite /kcas_casn_meta_size. lia. }
+                     rewrite -cons_seq.
+                     iDestruct "Hwitnesses" as "(Hwitness & Hwitnesses)".
+                     iEval (rewrite Nat.add_0_r) in "Hwitness".
+                     iDestruct (big_sepL_seq_shift_2 1 0 with "Hwitnesses") as "Hwitnesses".
+                     iEval (setoid_rewrite Nat.add_1_r) in "Hwitnesses".
+                     iEval (setoid_rewrite Nat.add_succ_r) in "Hwitnesses".
+                     assert (Nat.pred (kcas_casn_meta_size η - i) = kcas_casn_meta_size η - S i) as -> by lia.
+                     iSplitR "Hloc Hwitness HΦ". { do 2 iFrame. iSteps. }
+                     iModIntro. clear waiters.
+
+                     iSplitR "HΦ". { iFrame. iSteps. }
+                     iModIntro.
+
+                     wp_smart_apply ("Hdetermine_as" with "[$Hcasn_meta $Hcasn_inv' $Hlstatus_lb //] HΦ").
+
+               ++ iDestruct "Hlstatus" as "(%prophs & -> & Hlstatus)".
+                  iClear "Hlstatus_lb". iDestruct (kcas_lstatus_lb_get with "Hlstatus_auth") as "#Hlstatus_lb".
+                  iSplitR "HΦ". { do 2 iFrame. iSteps. }
+                  iModIntro. clear waiters prophs.
+
+                  rewrite /kcas_casn_meta_final.
+                  destruct (kcas_casn_meta_success η); iSteps.
+
+      - rewrite drop_lookup_None //.
+        { rewrite list_lookup_fmap Hdescrs_lookup //. }
+        wp_smart_apply (kcas_finish_spec_after with "[$Hcasn_meta $Hcasn_inv' $Hlstatus_lb]").
+        { rewrite lookup_ge_None in Hdescrs_lookup.
+          rewrite /kcas_casn_meta_size. lia.
+        }
+        iSteps.
+    }
+
+    { iIntros "%state %casn %η %descr !> %Φ (-> & %Hdescr & #Hcasn_meta & #Hcasn_inv') HΦ".
+
+      wp_recs credit:"H£".
+      wp_smart_apply ("Hdetermine" with "[$Hcasn_meta $Hcasn_inv']") as "#Hlstatus_lb".
+      rewrite /kcas_descr_final.
+      destruct (kcas_casn_meta_success η); iSteps.
+    }
+
+    { iIntros "%casn %η !> %Φ (#Hcasn_meta & #Hcasn_inv') HΦ".
+      iDestruct (kcas_casn_inv'_unfold with "Hcasn_inv'") as "(%P & #Hcasn_proph & #Hpost & %Hlocs & #Hcasn_inv & #Hlocs_inv)".
+
+      wp_recs.
+
+      wp_bind ((#casn).{status})%E.
+      iInv "Hcasn_inv" as "(%status & %lstatus & %waiters & Hcasn_status & Hlstatus_auth & Hwaiters_auth & Hlstatus)".
+      wp_load.
+      destruct lstatus as [i |].
+
+      - iDestruct "Hlstatus" as "(-> & Hlstatus)".
+        iDestruct (kcas_lstatus_lb_get_running0 with "Hlstatus_auth") as "#Hlstatus_lb".
+        iSplitR "HΦ". { do 2 iFrame. iSteps. }
+        iModIntro. clear.
+
+        wp_smart_apply ("Hdetermine_as" with "[$Hcasn_meta $Hcasn_inv' $Hlstatus_lb //]").
+        iSteps.
+
+      - iDestruct "Hlstatus" as "(%prophs & -> & Hlstatus)".
+        iDestruct (kcas_lstatus_lb_get with "Hlstatus_auth") as "#Hlstatus_lb".
+        iSplitR "HΦ". { do 2 iFrame. iSteps. }
+        iModIntro. clear.
+
+        rewrite /kcas_casn_meta_final.
+        destruct (kcas_casn_meta_success η); iSteps.
+    }
+  Admitted.
+  #[local] Lemma kcas_determine_as_spec casn η ι cass i :
     cass = lst_to_val (drop i (kcas_casn_meta_cass casn η)) →
     {{{
-      kcas_casn_inv' casn η ι ∗
-      kcas_lstatus_lb η (KcasUndetermined i) ∗
-      kcas_determine_specification
+      meta casn nroot η ∗
+      kcas_casn_inv' ι casn η ∗
+      kcas_lstatus_lb η (KcasRunning i)
     }}}
-      kcas_determine_aux #casn cass
+      kcas_determine_as #casn cass
     {{{
       RET #(kcas_casn_meta_success η);
       kcas_lstatus_lb η KcasFinished
     }}}.
   Proof.
-    iIntros (->) "%Φ (Hinv & #Hlstatus_lb & #Hdetermine) HΦ".
-
-    wp_recs.
-    wp_smart_apply (typed_prophet_wp_proph with "[//]") as (prophet prophs) "Hprophet".
-
-    destruct (kcas_casn_meta_cass casn η !! i) as [cas |] eqn:Hcass_lookup.
-
-    - erewrite drop_S; last done.
-      wp_pures.
-      admit.
-
-    -
-  Admitted.
-
+    iDestruct kcas_determine_as_get_as_determine_spec as "(H & _)".
+    iIntros (->) "%Φ (#Hcasn_meta & #Hcasn_inv' & #Hlstatus_lb) HΦ".
+    wp_apply ("H" with "[$Hcasn_meta $Hcasn_inv' $Hlstatus_lb //] HΦ").
+  Qed.
+  #[local] Lemma kcas_get_as_spec state casn η ι descr :
+    state = kcas_state casn descr →
+    descr ∈ η.(kcas_casn_meta_descrs) →
+    {{{
+      meta casn nroot η ∗
+      kcas_casn_inv' ι casn η
+    }}}
+      kcas_get_as state
+    {{{
+      RET kcas_descr_final descr η;
+      kcas_lstatus_lb η KcasFinished ∗
+      £ 1
+    }}}.
+  Proof.
+    iDestruct kcas_determine_as_get_as_determine_spec as "(_ & H & _)".
+    iIntros (-> Hdescr) "%Φ (#Hcasn_meta & #Hcasn_inv') HΦ".
+    wp_apply ("H" with "[$Hcasn_meta $Hcasn_inv' //] HΦ").
+  Qed.
   #[local] Lemma kcas_determine_spec casn η ι :
     {{{
-      kcas_casn_inv' casn η ι
+      meta casn nroot η ∗
+      kcas_casn_inv' ι casn η
     }}}
       kcas_determine #casn
     {{{
@@ -456,10 +1137,130 @@ Section kcas_G.
       kcas_lstatus_lb η KcasFinished
     }}}.
   Proof.
-  Admitted.
+    iDestruct kcas_determine_as_get_as_determine_spec as "(_ & _ & H)".
+    iIntros "%Φ (#Hcasn_meta & #Hcasn_inv') HΦ".
+    wp_apply ("H" with "[$Hcasn_meta $Hcasn_inv' //] HΦ").
+  Qed.
+
+  Lemma kcas_make_spec ι v :
+    {{{
+      True
+    }}}
+      kcas_make v
+    {{{ loc,
+      RET #loc;
+      kcas_loc_inv loc ι ∗
+      kcas_loc_model loc v
+    }}}.
+  Proof.
+    iIntros "%Φ _ HΦ".
+
+    wp_rec.
+    wp_apply (wp_id with "[//]") as (gid) "Hgid".
+    wp_smart_apply (typed_prophet_wp_proph kcas_prophet with "[//]") as (pid prophs) "Hproph_model".
+    wp_block casn as "Hcasn_meta" "(Hcasn_state & Hcasn_proph & _)".
+    iMod (pointsto_persist with "Hcasn_proph") as "#Hcasn_proph".
+    wp_reveal bid.
+    wp_ref loc as "Hloc_meta" "Hloc".
+
+    iMod kcas_model_alloc as "(%γ & Hmodel₁ & Hmodel₂)".
+
+    iMod (meta_set _ _ γ with "Hloc_meta") as "#Hloc_meta"; first done.
+
+    iMod (saved_prop_alloc True) as "(%η_post & #Hpost)".
+    iMod (kcas_lstatus_alloc KcasFinished) as "(%η_lstatus & Hlstatus_auth)".
+    iMod kcas_witness_alloc as "(%η_witness & Hwitness)".
+    iMod kcas_waiters_alloc as "(%η_waiters & Hwaiters_auth)".
+    iMod kcas_winning_alloc as "(%η_winning & Hwinning)".
+    iMod kcas_owner_alloc as "(%η_owner & Howner)".
+
+    pose descr := {|
+      kcas_descr_loc := loc ;
+      kcas_descr_meta := γ ;
+      kcas_descr_before := v ;
+      kcas_descr_after := v ;
+      kcas_descr_state := bid ;
+    |}.
+    pose η := {|
+      kcas_casn_meta_descrs := [descr] ;
+      kcas_casn_meta_prophet := pid ;
+      kcas_casn_meta_prophs := ((gid, true) :: prophs) ;
+      kcas_casn_meta_undetermined := bid ;
+      kcas_casn_meta_post := η_post ;
+      kcas_casn_meta_lstatus := η_lstatus ;
+      kcas_casn_meta_witnesses := [η_witness] ;
+      kcas_casn_meta_waiters := η_waiters ;
+      kcas_casn_meta_winning := η_winning ;
+      kcas_casn_meta_owner := η_owner ;
+    |}.
+    iMod (meta_set _ _ η with "Hcasn_meta") as "#Hcasn_meta"; first done.
+
+    iDestruct (kcas_lstatus_lb_get_finished (η := η) (KcasRunning 1) with "Hlstatus_auth") as "#Hlstatus_lb".
+
+    iMod (inv_alloc _ _ (kcas_casn_inv_inner casn η ι True) with "[Hgid Hproph_model Hcasn_state Hmodel₂ Hlstatus_auth Hwaiters_auth Hwinning Howner]") as "#Hcasn_inv".
+    { iExists KcasAfter, KcasFinished, ∅.
+      setoid_rewrite big_sepM_empty. iSteps.
+    }
+
+    iAssert (|={⊤}=> kcas_loc_inv' ι loc)%I with "[Hloc Hwitness]" as ">#Hloc_inv'".
+    { iApply kcas_loc_inv'_intro.
+      iApply inv_alloc.
+      iExists casn, η, 0, descr.
+      setoid_rewrite <- (fixpoint_A_unfold (kcas_casn_inv_pre ι) (kcas_loc_inv_pre ι) _).
+      iSteps. iPureIntro. apply NoDup_singleton.
+    }
+
+    iDestruct (kcas_casn_inv'_unfold with "[$Hcasn_inv]") as "#Hcasn_inv'".
+    { iSteps. iPureIntro. apply NoDup_singleton. }
+
+    iSteps.
+  Qed.
+
+  Lemma kcas_get_spec loc ι :
+    <<<
+      kcas_loc_inv loc ι
+    | ∀∀ v,
+      kcas_loc_model loc v
+    >>>
+      kcas_get #loc @ ↑ι
+    <<<
+      kcas_loc_model loc v
+    | RET v;
+      True
+    >>>.
+  Proof.
+    iIntros "!> %Φ (%γ & #Hloc_meta & #Hloc_inv') HΦ".
+    iDestruct (kcas_loc_inv'_elim with "Hloc_meta Hloc_inv'") as "#Hloc_inv".
+
+    wp_rec credit:"H£1".
+
+    wp_bind (!_)%E.
+    iInv "Hloc_inv" as "(%casn & %η & %i & %descr & #Hcasn_meta & >%Hdescrs_lookup & >-> & Hloc & #Hlstatus_lb & Hwitness & #Hcasn_inv')".
+    wp_load.
+    iDestruct (kcas_casn_inv'_unfold with "Hcasn_inv'") as "(%P & #Hcasn_proph & #Hpost & %Hlocs & #Hcasn_inv & #Hlocs_inv)".
+    iDestruct (big_sepL_lookup with "Hlocs_inv") as "(_Hloc_meta & _)"; first done.
+    iDestruct (meta_agree with "Hloc_meta _Hloc_meta") as %->. iClear "_Hloc_meta".
+    iMod (kcas_casn_wait _ _ (Φ (kcas_descr_final descr η)) with "Hcasn_inv Hwitness [HΦ]") as "(%waiter & Hwitness & #Hwaiter & Hwaiters_elem)"; [solve_ndisj | done.. | |].
+    { rewrite /kcas_waiter_au'. iAuIntro.
+      iApply (aacc_aupd_commit with "HΦ"); first done. iIntros "%v (%γ & _Hloc_meta & Hmodel₁)".
+      iDestruct (meta_agree with "Hloc_meta _Hloc_meta") as %<-. iClear "_Hloc_meta".
+      iAaccIntro with "Hmodel₁"; iSteps.
+    }
+    iSplitR "H£1 Hwaiters_elem". { iFrame. iSteps. }
+    iModIntro. clear Hlocs.
+
+    iApply wp_fupd. iClear "Hlstatus_lb".
+    wp_apply (kcas_get_as_spec with "[$Hcasn_meta $Hcasn_inv']") as "(#Hlstatus_lb & H£2)"; first done.
+    { eapply elem_of_list_lookup_2. done. }
+    iMod (kcas_casn_retrieve with "Hcasn_inv Hlstatus_lb Hwaiter Hwaiters_elem") as "HΦ".
+    iMod (lc_fupd_elim_later with "H£1 HΦ") as "HΦ".
+    iApply (lc_fupd_elim_later with "H£2 HΦ").
+  Qed.
 End kcas_G.
 
+#[global] Opaque kcas_make.
 #[global] Opaque kcas_get.
+#[global] Opaque kcas_cas.
 
 #[global] Opaque kcas_loc_inv.
 #[global] Opaque kcas_loc_model.
